@prefix : <http://data.europa.eu/2sa/cav#> .
@prefix cc: <http://creativecommons.org/ns#> .
@prefix dc: <http://www.omg.org/spec/UML/20131001/UMLDC> .
@prefix cav: <http://data.europa.eu/2sa/cav#> .
@prefix dct: <http://purl.org/dc/terms/> .
@prefix org: <http://www.w3.org/ns/org#> .
@prefix owl: <http://www.w3.org/2002/07/owl#> .
@prefix pav: <http://purl.org/pav/> .
@prefix rdf: <http://www.w3.org/1999/02/22-rdf-syntax-ns#> .
@prefix sch: <https://schema.org/> .
@prefix xml: <http://www.w3.org/XML/1998/namespace> .
@prefix xsd: <http://www.w3.org/2001/XMLSchema#> .
@prefix dcat: <http://www.w3.org/ns/dcat#> .
@prefix foaf: <http://xmlns.com/foaf/0.1/> .
@prefix rdfs: <http://www.w3.org/2000/01/rdf-schema#> .
@prefix skos: <http://www.w3.org/2004/02/skos/core#> .
@prefix vann: <http://purl.org/vocab/vann/> .
@prefix cccev: <https://data.europe.eu/semanticassets/ns/cv/cccev_v2.0.0#> .
@base <http://data.europa.eu/2sa/cav#> .

<http://data.europa.eu/2sa/cav#> rdf:type owl:Ontology ;
                                  owl:versionIRI cav:CAV.xml-2022-07-25 ;
                                  owl:imports dct: ,
                                              rdfs: ,
                                              <http://www.w3.org/2004/02/skos/core> ,
                                              dcat: ,
                                              foaf: ;
                                  cc:attributionName "European Commission" ;
                                  dct:date "2020-11-18+01:00"^^xsd:date ;
                                  dct:description "This module provides the definitions for the Core Assessment Vocabulary."@en ;
                                  dct:license <http://creativecommons.org/licenses/by-sa/4.0/> ;
                                  dct:title "Core Assessment Vocabulary"@en ;
                                  vann:preferredNamespacePrefix "cav" ;
                                  vann:preferredNamespaceUri "http://data.europa.eu/2sa/cav#" ;
                                  rdfs:label "Core Assessment Vocabulary"@en ;
                                  rdfs:seeAlso <https://github.com/isa-camss/CAV> ,
                                               <https://joinup.ec.europa.eu/collection/common-assessment-method-standards-and-specifications-camss/solution/core-assessment-vocabulary-cav> ;
                                  owl:versionInfo "1.2.0" ;
                                  skos:note "This file has been generated with the tool developed by the Publications Office of the European Union, which takes the UML representation of the core vocabulary as a basis"@en .

#################################################################
#    Annotation properties
#################################################################

###  http://creativecommons.org/ns#attributionName
cc:attributionName rdf:type owl:AnnotationProperty .


###  http://purl.org/dc/terms/date
dct:date rdf:type owl:AnnotationProperty .


###  http://purl.org/dc/terms/description
dct:description rdf:type owl:AnnotationProperty .


###  http://purl.org/dc/terms/license
dct:license rdf:type owl:AnnotationProperty .


###  http://purl.org/dc/terms/title
dct:title rdf:type owl:AnnotationProperty .


###  http://purl.org/vocab/vann/preferredNamespacePrefix
vann:preferredNamespacePrefix rdf:type owl:AnnotationProperty .


###  http://purl.org/vocab/vann/preferredNamespaceUri
vann:preferredNamespaceUri rdf:type owl:AnnotationProperty .


###  http://www.w3.org/2004/02/skos/core#altLabel
skos:altLabel rdf:type owl:AnnotationProperty .


###  http://www.w3.org/2004/02/skos/core#definition
skos:definition rdf:type owl:AnnotationProperty .


###  http://www.w3.org/2004/02/skos/core#note
skos:note rdf:type owl:AnnotationProperty .


###  http://www.w3.org/2004/02/skos/core#prefLabel
skos:prefLabel rdf:type owl:AnnotationProperty .


###  http://www.w3.org/2004/02/skos/core#scopeNote
skos:scopeNote rdf:type owl:AnnotationProperty .


#################################################################
#    Datatypes
#################################################################

###  http://www.w3.org/2001/XMLSchema#date
xsd:date rdf:type rdfs:Datatype .


###  http://www.w3.org/2004/02/skos/core#Concept
skos:Concept rdf:type rdfs:Datatype .


#################################################################
#    Object Properties
#################################################################

###  http://data.europa.eu/2sa/cav#assesses
cav:assesses rdf:type owl:ObjectProperty ;
             rdfs:domain cav:Assessment ;
             rdfs:range dcat:Resource ;
             rdfs:comment "The reference to the asset(s) that are the object of the assessment.  (cav:Assessment -> dcat:Resource (+cav:assesses)) "@en ;
             rdfs:isDefinedBy <http://data.europa.eu/w21/2c930c7b-5e2f-4954-8522-bd3411339d6c> ;
             rdfs:label "Assesses"@en ;
             skos:definition "The reference to the asset(s) that are the object of the assessment.  (cav:Assessment -> dcat:Resource (+cav:assesses)) "@en ;
             skos:prefLabel "Assesses"@en .


###  http://data.europa.eu/2sa/cav#assignedTo
cav:assignedTo rdf:type owl:ObjectProperty ;
               rdfs:domain cav:Score ;
               rdfs:range cccev:Criterion ;
               rdfs:comment "The assignment of a value output to the criterion.  (cav:Score <-> cccev:Criterion (+cav:assignedTo +)) "@en ;
               rdfs:isDefinedBy <http://data.europa.eu/w21/2c930c7b-5e2f-4954-8522-bd3411339d6c> ;
               rdfs:label "Assigned to"@en ;
               skos:definition "The assignment of a value output to the criterion.  (cav:Score <-> cccev:Criterion (+cav:assignedTo +)) "@en ;
               skos:prefLabel "Assigned to"@en .


###  http://data.europa.eu/2sa/cav#basedOn
cav:basedOn rdf:type owl:ObjectProperty ;
            rdfs:domain cav:Score ;
            rdfs:range cav:EvaluationContext ;
            rdfs:comment "The consideration of a specific evaluation context when assigning the score to a criterion. (cav:Score -> cav:EvaluationContext (+cav:basedOn)) "@en ;
            rdfs:isDefinedBy <http://data.europa.eu/w21/2c930c7b-5e2f-4954-8522-bd3411339d6c> ;
            rdfs:label "Based on"@en ;
            skos:definition "The consideration of a specific evaluation context when assigning the score to a criterion. (cav:Score -> cav:EvaluationContext (+cav:basedOn)) "@en ;
            skos:prefLabel "Based on"@en .


###  http://data.europa.eu/2sa/cav#considers
cav:considers rdf:type owl:ObjectProperty ;
              rdfs:domain cav:Assessment ;
              rdfs:range cav:Score ;
              rdfs:comment "The evaluation of a criterion score in the context of the current assessment as input to issue one or more statements."@en ;
              rdfs:isDefinedBy <http://data.europa.eu/w21/2c930c7b-5e2f-4954-8522-bd3411339d6c> ;
              rdfs:label "Considers"@en ;
              skos:definition "The evaluation of an assessment score as input to issue one or more statements."@en ;
              skos:prefLabel "Considers"@en .


###  http://data.europa.eu/2sa/cav#contextualisedBy
cav:contextualisedBy rdf:type owl:ObjectProperty ;
                     rdfs:domain cav:Assessment ;
                     rdfs:range cav:Scenario ;
                     rdfs:comment "The assignment of the scenario for the current assessment providing its context, purpose and criteria."@en ;
                     rdfs:isDefinedBy <http://data.europa.eu/w21/2c930c7b-5e2f-4954-8522-bd3411339d6c> ;
                     rdfs:label "Contextualised by"@en ;
                     skos:definition "The assignment of the scenario for the current assessment providing its context, purpose and criteria."@en ;
                     skos:prefLabel "Contextualised by"@en .


###  http://data.europa.eu/2sa/cav#contextualises
cav:contextualises rdf:type owl:ObjectProperty ;
                   rdfs:domain cav:EvaluationContext ;
                   rdfs:range cccev:Criterion ;
                   rdfs:comment "The provision of context for the evaluation of the criterion."@en ;
                   rdfs:isDefinedBy <http://data.europa.eu/w21/2c930c7b-5e2f-4954-8522-bd3411339d6c> ;
                   rdfs:label "Contextualises"@en ;
                   skos:definition "The provision of context for the evaluation of the criterion."@en ;
                   skos:prefLabel "Contextualises"@en .


###  http://data.europa.eu/2sa/cav#definedBy
cav:definedBy rdf:type owl:ObjectProperty ;
              owl:inverseOf cav:defines ;
              rdfs:domain cav:EvaluationContext ;
              rdfs:range cav:Scenario ;
              rdfs:comment "The link to the scenario that provides the evaluation context for one or more criteria"@en ;
              rdfs:isDefinedBy <http://data.europa.eu/w21/2c930c7b-5e2f-4954-8522-bd3411339d6c> ;
              rdfs:label "Defined by"@en ;
              skos:definition "The link to the scenario that provides the evaluation context for one or more criteria."@en ;
              skos:prefLabel "Defined by"@en .


###  http://data.europa.eu/2sa/cav#defines
cav:defines rdf:type owl:ObjectProperty ;
            rdfs:domain cav:Scenario ;
            rdfs:range cav:EvaluationContext ;
            rdfs:comment "The link to the evaluation contexts for specific criteria provided by the given scenario."@en ;
            rdfs:isDefinedBy <http://data.europa.eu/w21/2c930c7b-5e2f-4954-8522-bd3411339d6c> ;
            rdfs:label "Defines"@en ;
            skos:definition "The link to the evaluation contexts for specific criteria provided by the given scenario."@en ;
            skos:prefLabel "Defines"@en .


###  http://data.europa.eu/2sa/cav#definesSub
cav:definesSub rdf:type owl:ObjectProperty ;
               rdfs:domain cav:Scenario ;
               rdfs:range cav:Scenario ;
               rdfs:comment "The definition of nested scenarios grouped based on different sub-purposes, commonalities or particularities of the sub-sets of criteria."@en ;
               rdfs:isDefinedBy <http://data.europa.eu/w21/2c930c7b-5e2f-4954-8522-bd3411339d6c> ;
               rdfs:label "Defines sub"@en ;
               skos:definition "The definition of nested scenarios grouped based on different sub-purposes, commonalities or particularities of the sub-sets of criteria."@en ;
               skos:prefLabel "Defines sub"@en .


###  http://data.europa.eu/2sa/cav#documentedIn
cav:documentedIn rdf:type owl:ObjectProperty ;
                 rdfs:domain cav:Asset ;
                 rdfs:range rdfs:Resource ;
                 rdfs:comment "A link to any information supporting the value of the asset and any other related relevant details."@en ;
                 rdfs:isDefinedBy <http://data.europa.eu/w21/2c930c7b-5e2f-4954-8522-bd3411339d6c> ;
                 rdfs:label "Documented in"@en ;
                 skos:definition "A link to any information supporting the value of the asset and any other related relevant details."@en ;
                 skos:prefLabel "Documented in"@en .


###  http://data.europa.eu/2sa/cav#formulatedBy
cav:formulatedBy rdf:type owl:ObjectProperty ;
                 rdfs:domain cav:Statement ;
                 rdfs:range foaf:Agent ;
                 rdfs:comment "The agent(s) that issue value judgement(s) resulting from the assessment."@en ;
                 rdfs:isDefinedBy <http://data.europa.eu/w21/2c930c7b-5e2f-4954-8522-bd3411339d6c> ;
                 rdfs:label "Formulated by"@en ;
                 skos:definition "The agent(s) that issue value judgement(s) resulting from the assessment."@en ;
                 skos:prefLabel "Formulated by"@en .


###  http://data.europa.eu/2sa/cav#hasInput
cav:hasInput rdf:type owl:ObjectProperty ;
             rdfs:domain cav:Score ;
             rdfs:range rdfs:Resource ;
             rdfs:comment "The different resources provided to feed the context for the evaluation of a criterion."@en ;
             rdfs:isDefinedBy <http://data.europa.eu/w21/2c930c7b-5e2f-4954-8522-bd3411339d6c> ;
             rdfs:label "Has input"@en ;
             skos:definition "The different resources provided to feed the context for the evaluation of a criterion. "@en ;
             skos:prefLabel "Has input"@en .


###  http://data.europa.eu/2sa/cav#hasReport
cav:hasReport rdf:type owl:ObjectProperty ;
              rdfs:domain cav:Assessment ;
              rdfs:range dcat:Distribution ;
              rdfs:comment "A manifestation of all the information related to and resulting from an assessment."@en ;
              rdfs:isDefinedBy <http://data.europa.eu/w21/2c930c7b-5e2f-4954-8522-bd3411339d6c> ;
              rdfs:label "Has report"@en ;
              skos:definition "A manifestation of all the information related to and resulting from an assessment."@en ;
              skos:prefLabel "Has report"@en .


###  http://data.europa.eu/2sa/cav#hasSummary
cav:hasSummary rdf:type owl:ObjectProperty ;
               rdfs:domain cav:Assessment ;
               rdfs:range dcat:Distribution ;
               rdfs:comment "An abbreviated manifestation of the performed assessment."@en ;
               rdfs:isDefinedBy <http://data.europa.eu/w21/2c930c7b-5e2f-4954-8522-bd3411339d6c> ;
               rdfs:label "Has summary"@en ;
               skos:definition "An abbreviated manifestation of the performed assessment."@en ;
               skos:prefLabel "Has summary"@en .


###  http://data.europa.eu/2sa/cav#includes
cav:includes rdf:type owl:ObjectProperty ;
             rdfs:domain cav:Scenario ;
             rdfs:range cccev:Criterion ;
             rdfs:comment "The aggregation of criteria to one scenario or parts of it."@en ;
             rdfs:isDefinedBy <http://data.europa.eu/w21/2c930c7b-5e2f-4954-8522-bd3411339d6c> ;
             rdfs:label "Includes"@en ;
             skos:definition "The aggregation of criteria to one scenario or parts of it."@en ;
             skos:prefLabel "Includes"@en .


###  http://data.europa.eu/2sa/cav#performedBy
cav:performedBy rdf:type owl:ObjectProperty ;
                rdfs:domain cav:Assessment ;
                rdfs:range foaf:Agent ;
                rdfs:comment "The agent(s) that carry out the assessment."@en ;
                rdfs:isDefinedBy <http://data.europa.eu/w21/2c930c7b-5e2f-4954-8522-bd3411339d6c> ;
                rdfs:label "Performed by"@en ;
                skos:definition "The agent(s) that carry out the assessment."@en ;
                skos:prefLabel "Performed by"@en .


###  http://data.europa.eu/2sa/cav#providedBy
cav:providedBy rdf:type owl:ObjectProperty ;
               owl:inverseOf cav:providesScore ;
               rdfs:domain cav:Score ;
               rdfs:range foaf:Agent ;
               rdfs:comment "The agent assigning the score for a given criterion as part of the assessment."@en ;
               rdfs:isDefinedBy <http://data.europa.eu/w21/2c930c7b-5e2f-4954-8522-bd3411339d6c> ;
               rdfs:label "Provided by"@en ;
               skos:definition "The agent assigning the score for a given criterion as part of the assessment."@en ;
               skos:prefLabel "Provided by"@en .


###  http://data.europa.eu/2sa/cav#providesScore
cav:providesScore rdf:type owl:ObjectProperty ;
                  rdfs:domain foaf:Agent ;
                  rdfs:range cav:Score ;
                  rdfs:comment "The agent assigning the score for a given criterion as part of the assessment."@en ;
                  rdfs:isDefinedBy <http://data.europa.eu/w21/2c930c7b-5e2f-4954-8522-bd3411339d6c> ;
                  rdfs:label "Provides score"@en ;
                  skos:definition "The agent assigning the score for a given criterion as part of the assessment."@en ;
                  skos:prefLabel "Provides score"@en .


###  http://data.europa.eu/2sa/cav#refersTo
cav:refersTo rdf:type owl:ObjectProperty ;
             rdfs:domain cav:Statement ;
             rdfs:range cav:Scenario ,
                        cav:Score ,
                        cccev:Criterion ;
             rdfs:comment "The provision of a value judgement on one or more elements of the assessment."@en ;
             rdfs:isDefinedBy <http://data.europa.eu/w21/2c930c7b-5e2f-4954-8522-bd3411339d6c> ;
             rdfs:label "Refers to"@en ;
             skos:definition "The provision of a value judgement on one or more elements of the assessment."@en ;
             skos:prefLabel "Refers to"@en .


###  http://data.europa.eu/2sa/cav#relatesTo
cav:relatesTo rdf:type owl:ObjectProperty ;
              rdfs:domain cav:EvaluationContext ;
              rdfs:range rdfs:Resource ;
              rdfs:comment "The resource to which a domain concept relates to."@en ;
              rdfs:isDefinedBy <http://data.europa.eu/w21/2c930c7b-5e2f-4954-8522-bd3411339d6c> ;
              rdfs:label "Relates to"@en ;
              skos:definition "The resource to which a domain concept relates to."@en ;
              skos:prefLabel "Relates to"@en .


###  http://data.europa.eu/2sa/cav#requestedBy
cav:requestedBy rdf:type owl:ObjectProperty ;
                rdfs:domain cav:Assessment ;
                rdfs:range foaf:Agent ;
                rdfs:comment "The agent(s) requesting the assessment of an asset."@en ;
                rdfs:isDefinedBy <http://data.europa.eu/w21/2c930c7b-5e2f-4954-8522-bd3411339d6c> ;
                rdfs:label "Requested by"@en ;
                skos:definition "The agent(s) requesting the assessment of an asset."@en ;
                skos:prefLabel "Requested by"@en .


###  http://data.europa.eu/2sa/cav#resultsIn
cav:resultsIn rdf:type owl:ObjectProperty ;
              rdfs:domain cav:Assessment ;
              rdfs:range cav:Statement ;
              rdfs:comment "The creation of the statements resulting from the assessment."@en ;
              rdfs:isDefinedBy <http://data.europa.eu/w21/2c930c7b-5e2f-4954-8522-bd3411339d6c> ;
              rdfs:label "Results in"@en ;
              skos:definition "The creation of the statements resulting from the assessment."@en ;
              skos:prefLabel "Results in"@en .


###  http://data.europa.eu/2sa/cav#triggeredFrom
cav:triggeredFrom rdf:type owl:ObjectProperty ;
                  owl:inverseOf cav:triggers ;
                  rdfs:domain cav:Assessment ;
                  rdfs:range cav:Assessment ;
                  rdfs:comment "The event causing the current assessment as the result of another related assessment."@en ;
                  rdfs:isDefinedBy <http://data.europa.eu/w21/2c930c7b-5e2f-4954-8522-bd3411339d6c> ;
                  rdfs:label "Triggered from"@en ;
                  skos:definition "The event causing the current assessment as the result of another related assessment."@en ;
                  skos:prefLabel "Triggered from"@en .


###  http://data.europa.eu/2sa/cav#triggers
cav:triggers rdf:type owl:ObjectProperty ;
             rdfs:domain cav:Assessment ;
             rdfs:range cav:Assessment ;
             rdfs:comment "The event causing further related assessment(s) due to the current one."@en ;
             rdfs:isDefinedBy <http://data.europa.eu/w21/2c930c7b-5e2f-4954-8522-bd3411339d6c> ;
             rdfs:label "Triggers"@en ;
             skos:definition "The event causing further related assessment(s) due to the current one."@en ;
             skos:prefLabel "Triggers"@en .


###  http://purl.org/dc/terms/creator
dct:creator rdf:type owl:ObjectProperty ;
            rdfs:domain dcat:Resource ;
            rdfs:range foaf:Agent ;
            rdfs:comment "The entity responsible for producing the resource."@en ;
            rdfs:isDefinedBy <https://www.dublincore.org/specifications/dublin-core/dcmi-terms/> ;
            rdfs:label "Creator"@en ;
            skos:definition "The entity responsible for producing the resource."@en ;
            skos:prefLabel "Creator"@en .


###  http://purl.org/pav/previousVersion
pav:previousVersion rdf:type owl:ObjectProperty ;
                    rdfs:domain cav:Assessment ;
                    rdfs:range cav:Assessment ;
                    rdfs:comment "The previous version of a resource in a lineage."@en ;
                    rdfs:isDefinedBy pav: ;
                    rdfs:label "Previous version"@en ;
                    skos:definition "The previous version of a resource in a lineage."@en ;
                    skos:prefLabel "Previous version"@en .


###  http://www.w3.org/ns/dcat#distribution
dcat:distribution rdf:type owl:ObjectProperty ;
                  rdfs:domain dcat:Dataset ;
                  rdfs:range dcat:Distribution ;
                  rdfs:comment "An available distribution of the dataset."@en ;
                  rdfs:isDefinedBy <https://www.w3.org/ns/dcat> ;
                  rdfs:label "Distribution"@en ;
                  skos:definition "An available distribution of the dataset."@en ;
                  skos:prefLabel "Distribution"@en .


###  https://schema.org/contactPoint
sch:contactPoint rdf:type owl:ObjectProperty ;
                 rdfs:domain sch:ContactPoint ;
                 rdfs:range org:Organization ;
                 rdfs:comment "A contact point for a person or organization."@en ;
                 rdfs:isDefinedBy <https://schema.org/docs/schemas.html> ;
                 rdfs:label "Contact Point"@en ;
                 skos:definition "A contact point for a person or organization."@en ;
                 skos:prefLabel "Contact Point"@en .


#################################################################
#    Data properties
#################################################################

###  http://data.europa.eu/2sa/cav#instructionDescription
cav:instructionDescription rdf:type owl:DatatypeProperty ;
                           rdfs:domain cav:EvaluationContext ;
                           rdfs:range xsd:string ;
                           rdfs:comment "Guideline or description that needs to followed during the evaluation of one particular criterion."@en ;
                           rdfs:isDefinedBy <http://data.europa.eu/w21/2c930c7b-5e2f-4954-8522-bd3411339d6c> ;
                           rdfs:label "Instruction description"@en ;
                           skos:altLabel "Has instruction description"@en ;
                           skos:definition "Guideline or description that needs to followed during the evaluation of one particular criterion."@en ;
                           skos:prefLabel "Instruction description"@en .


###  http://data.europa.eu/2sa/cav#interpretation
cav:interpretation rdf:type owl:DatatypeProperty ;
                   rdfs:domain cav:Statement ;
                   rdfs:range skos:Concept ;
                   rdfs:comment "The favourability perception of the statement (e.g. positive, negative or neutral)."@en ;
                   rdfs:isDefinedBy <http://data.europa.eu/w21/2c930c7b-5e2f-4954-8522-bd3411339d6c> ;
                   rdfs:label "Interpretation"@en ;
                   skos:altLabel "Has interpretation"@en ;
                   skos:definition "The favourability perception of the statement (e.g. positive, negative or neutral)."@en ;
                   skos:prefLabel "Interpretation"@en .


###  http://data.europa.eu/2sa/cav#judgement
cav:judgement rdf:type owl:DatatypeProperty ;
              rdfs:domain cav:Statement ;
              rdfs:range xsd:string ;
              rdfs:comment "The text expressing the statement’s resulting value judgement. (cav:Statement) "@en ;
              rdfs:isDefinedBy <http://data.europa.eu/w21/2c930c7b-5e2f-4954-8522-bd3411339d6c> ;
              rdfs:label "Judgement"@en ;
              skos:altLabel "Has judgement"@en ;
              skos:definition "The text expressing the statement’s resulting value judgement. (cav:Statement) "@en ;
              skos:prefLabel "Judgement"@en .


###  http://data.europa.eu/2sa/cav#purpose
cav:purpose rdf:type owl:DatatypeProperty ;
            rdfs:domain cav:Scenario ;
            rdfs:range xsd:string ;
            rdfs:comment "The reason for which the assessment is done."@en ;
            rdfs:isDefinedBy <http://data.europa.eu/w21/2c930c7b-5e2f-4954-8522-bd3411339d6c> ;
            rdfs:label "Purpose"@en ;
            skos:altLabel "Has purpose"@en ;
            skos:definition "The reason for which the assessment is done."@en ;
            skos:prefLabel "Purpose"@en .


###  http://data.europa.eu/2sa/cav#status
cav:status rdf:type owl:DatatypeProperty ;
           rdfs:domain cav:Assessment ;
           rdfs:range skos:Concept ;
           rdfs:comment "The current situation of the assessment."@en ;
           rdfs:isDefinedBy <http://data.europa.eu/w21/2c930c7b-5e2f-4954-8522-bd3411339d6c> ;
           rdfs:label "Status"@en ;
           skos:altLabel "Has label"@en ;
           skos:definition "The current situation of the assessment."@en ;
           skos:prefLabel "Status"@en .


###  http://data.europa.eu/2sa/cav#type
cav:type rdf:type owl:DatatypeProperty ;
         rdfs:comment "The categorisation of the statement."@en ;
         rdfs:isDefinedBy <http://data.europa.eu/w21/2c930c7b-5e2f-4954-8522-bd3411339d6c> ;
         rdfs:label "Type"@en ;
         skos:altLabel "Has type"@en ;
         skos:definition "The categorisation of the statement."@en ;
         skos:prefLabel "Type"@en .


###  http://data.europa.eu/2sa/cav#value
cav:value rdf:type owl:DatatypeProperty ;
          rdfs:domain cav:Score ;
          rdfs:range rdfs:Literal ;
          rdfs:comment "The literal representing the final score assigned to one criterion."@en ;
          rdfs:isDefinedBy <http://data.europa.eu/w21/2c930c7b-5e2f-4954-8522-bd3411339d6c> ;
          rdfs:label "Value"@en ;
          skos:altLabel "Has value"@en ;
          skos:definition "The literal representing the score assigned."@en ;
          skos:prefLabel "Value"@en .


###  http://data.europa.eu/2sa/cav#valueDescription
cav:valueDescription rdf:type owl:DatatypeProperty ;
                     rdfs:domain cav:Asset ;
                     rdfs:range xsd:string ;
                     rdfs:comment "A text explaining the value of the resource being assessed in the context of a particular scenario."@en ;
                     rdfs:isDefinedBy <http://data.europa.eu/w21/2c930c7b-5e2f-4954-8522-bd3411339d6c> ;
                     rdfs:label "Value description"@en ;
                     skos:altLabel "Has value description"@en ;
                     skos:definition "A text explaining the value of the resource being assessed in the context of a particular scenario."@en ;
                     skos:prefLabel "Value Description"@en .


###  http://purl.org/dc/terms/issued
dct:issued rdf:type owl:DatatypeProperty ;
           rdfs:domain dcat:Resource ;
           rdfs:range xsd:string ;
           rdfs:comment "Recommended practice is to describe the date, date/time, or period of time as recommended for the property Date, of which this is a subproperty."@en ;
           rdfs:isDefinedBy <https://www.dublincore.org/specifications/dublin-core/dcmi-terms/> ;
           rdfs:label "Date issued"@en ;
           skos:definition "Date of formal issuance of the resource."@en ;
           skos:prefLabel "Date issued"@en .


###  http://purl.org/pav/version
pav:version rdf:type owl:DatatypeProperty ;
            rdfs:domain cav:Assessment ;
            rdfs:range xsd:string ;
            rdfs:comment "The version number of a resource. This is a freetext string, typical values are \"1.5\" or \"21\". The URI identifying the previous version can be provided using prov:previousVersion."@en ;
            rdfs:isDefinedBy pav: ;
            rdfs:label "Previous version"@en ;
            skos:definition "The version number of a resource. This is a freetext string, typical values are \"1.5\" or \"21\". The URI identifying the previous version can be provided using prov:previousVersion."@en ;
            skos:prefLabel "Previous version"@en .


#################################################################
#    Classes
#################################################################

###  http://data.europa.eu/2sa/cav#Assessment
cav:Assessment rdf:type owl:Class ;
               rdfs:subClassOf cav:Asset ;
               rdfs:comment "The intellectual work to evaluate an asset against the criteria of a given scenario."@en ;
               rdfs:isDefinedBy <http://data.europa.eu/w21/2c930c7b-5e2f-4954-8522-bd3411339d6c> ;
               rdfs:label "Assessment"@en ;
               skos:definition "The intellectual work to evaluate an asset against the criteria of a given scenario."@en ;
               skos:prefLabel "Assessment"@en .


###  http://data.europa.eu/2sa/cav#Asset
cav:Asset rdf:type owl:Class ;
          rdfs:subClassOf dcat:Resource ;
          rdfs:comment "A resource, probably resulting from a work, with purpose and value."@en ;
          rdfs:isDefinedBy <http://data.europa.eu/w21/2c930c7b-5e2f-4954-8522-bd3411339d6c> ;
          rdfs:label "Asset"@en ;
          skos:definition "A resource, probably resulting from a work, with purpose and value."@en ;
          skos:prefLabel "Asset"@en .


###  http://data.europa.eu/2sa/cav#EvaluationContext
cav:EvaluationContext rdf:type owl:Class ;
                      rdfs:comment "The context for a criterion providing guidance on its evaluation considering the given scenario. This is used exceptionally to extend the context offered by the scenario when it is not sufficient for the evaluation of a given criterion. An criterion's evaluation produces an objective output that will then be considered to form value judgments expressed as the assessment's statements."@en ;
                      rdfs:isDefinedBy <http://data.europa.eu/w21/2c930c7b-5e2f-4954-8522-bd3411339d6c> ;
                      rdfs:label "Evaluation context"@en ;
                      skos:definition "The context for a criterion providing guidance on its evaluation considering the given scenario. This is used exceptionally to extend the context offered by the scenario when it is not sufficient for the evaluation of a given criterion. An criterion's evaluation produces an objective output that will then be considered to form value judgments expressed as the assessment's statements."@en ;
                      skos:prefLabel "Evaluation context"@en .


###  http://data.europa.eu/2sa/cav#Scenario
cav:Scenario rdf:type owl:Class ;
             rdfs:subClassOf dcat:Resource ;
             owl:disjointWith dcat:Dataset ;
             rdfs:comment "The context of the assessment establishing its purpose, the organisation of criteria being evaluated, and its reference frameworks."@en ;
             rdfs:isDefinedBy <http://data.europa.eu/w21/2c930c7b-5e2f-4954-8522-bd3411339d6c> ;
             rdfs:label "Scenario"@en ;
             skos:definition "The context of the assessment establishing its purpose, the organisation of criteria being evaluated, and its reference frameworks."@en ;
             skos:prefLabel "Scenario"@en .


###  http://data.europa.eu/2sa/cav#Score
cav:Score rdf:type owl:Class ;
          rdfs:comment "The value output assigned to the criterion as part of the assessment."@en ;
          rdfs:isDefinedBy <http://data.europa.eu/w21/2c930c7b-5e2f-4954-8522-bd3411339d6c> ;
          rdfs:label "Score"@en ;
          skos:definition "The value output assigned to the criteria as part of the assessment. Additional info: This value output can be individual, and therefore per criterion or global representing the overall score of the assessment (e.g. In the case of CAMSS, assessments include two different scores)."@en ;
          skos:prefLabel "Score"@en .


###  http://data.europa.eu/2sa/cav#Statement
cav:Statement rdf:type owl:Class ;
              rdfs:comment "A value judgement, resulting from the assessment, pertinent to its entirety or to one or more of its specific parts."@en ;
              rdfs:isDefinedBy <http://data.europa.eu/w21/2c930c7b-5e2f-4954-8522-bd3411339d6c> ;
              rdfs:label "Statement"@en ;
              skos:definition "A value judgement, resulting from the assessment, pertinent to its entirety or to one or more of its specific parts."@en ;
              skos:prefLabel "Statement"@en .


###  http://www.w3.org/2000/01/rdf-schema#Resource
rdfs:Resource rdf:type owl:Class .


###  http://www.w3.org/ns/dcat#Dataset
dcat:Dataset rdf:type owl:Class ;
             rdfs:subClassOf dcat:Resource .


###  http://www.w3.org/ns/dcat#Distribution
dcat:Distribution rdf:type owl:Class .


###  http://www.w3.org/ns/dcat#Resource
dcat:Resource rdf:type owl:Class .


###  http://www.w3.org/ns/org#Organization
org:Organization rdf:type owl:Class ;
                 rdfs:subClassOf foaf:Agent .


###  http://xmlns.com/foaf/0.1/Agent
foaf:Agent rdf:type owl:Class .


###  https://data.europe.eu/semanticassets/ns/cv/cccev_v2.0.0#Criterion
cccev:Criterion rdf:type owl:Class .


###  https://schema.org/ContactPoint
sch:ContactPoint rdf:type owl:Class .


###  Generated by the OWL API (version 4.5.25.2023-02-15T19:15:49Z) https://github.com/owlcs/owlapi
