<?xml version="1.0"?>
<rdf:RDF xmlns="http://data.europa.eu/2sa/cav#"
     xml:base="http://data.europa.eu/2sa/cav"
     xmlns:cc="http://creativecommons.org/ns#"
     xmlns:dc="http://purl.org/dc/elements/1.1/"
     xmlns:ns="http://www.w3.org/2003/06/sw-vocab-status/ns#"
     xmlns:cav="http://data.europa.eu/2sa/cav#"
     xmlns:dct="http://purl.org/dc/terms/"
     xmlns:org="http://www.w3.org/ns/org#"
     xmlns:owl="http://www.w3.org/2002/07/owl#"
     xmlns:pav="http://purl.org/pav/"
     xmlns:rdf="http://www.w3.org/1999/02/22-rdf-syntax-ns#"
     xmlns:sch="https://schema.org/"
     xmlns:wot="http://xmlns.com/wot/0.1/"
     xmlns:xml="http://www.w3.org/XML/1998/namespace"
     xmlns:xsd="http://www.w3.org/2001/XMLSchema#"
     xmlns:dcat="http://www.w3.org/ns/dcat#"
     xmlns:foaf="http://xmlns.com/foaf/0.1/"
     xmlns:rdfs="http://www.w3.org/2000/01/rdf-schema#"
     xmlns:skos="http://www.w3.org/2004/02/skos/core#"
     xmlns:vann="http://purl.org/vocab/vann/"
     xmlns:cccev="https://data.europe.eu/semanticassets/ns/cv/cccev_v2.0.0#">
    <owl:Ontology rdf:about="http://data.europa.eu/2sa/cav#">
        <owl:versionIRI rdf:resource="http://data.europa.eu/2sa/cav#CAV.xml-2022-07-25"/>
        <owl:imports rdf:resource="http://purl.org/dc/terms/"/>
        <owl:imports rdf:resource="http://www.w3.org/2000/01/rdf-schema#"/>
        <owl:imports rdf:resource="http://www.w3.org/2004/02/skos/core"/>
        <owl:imports rdf:resource="http://www.w3.org/ns/dcat#"/>
        <owl:imports rdf:resource="http://xmlns.com/foaf/0.1/"/>
        <cc:attributionName>European Commission</cc:attributionName>
        <dct:date rdf:datatype="http://www.w3.org/2001/XMLSchema#date">2020-11-18+01:00</dct:date>
        <dct:description xml:lang="en">This module provides the definitions for the Core Assessment Vocabulary.</dct:description>
        <dct:license rdf:resource="http://creativecommons.org/licenses/by-sa/4.0/"/>
        <dct:title xml:lang="en">Core Assessment Vocabulary</dct:title>
        <vann:preferredNamespacePrefix>cav</vann:preferredNamespacePrefix>
        <vann:preferredNamespaceUri>http://data.europa.eu/2sa/cav#</vann:preferredNamespaceUri>
        <rdfs:label xml:lang="en">Core Assessment Vocabulary</rdfs:label>
        <rdfs:seeAlso rdf:resource="https://github.com/isa-camss/CAV"/>
        <rdfs:seeAlso rdf:resource="https://joinup.ec.europa.eu/collection/common-assessment-method-standards-and-specifications-camss/solution/core-assessment-vocabulary-cav"/>
        <owl:versionInfo>1.2.0</owl:versionInfo>
        <skos:note xml:lang="en">This file has been generated with the tool developed by the Publications Office of the European Union, which takes the UML representation of the core vocabulary as a basis</skos:note>
    </owl:Ontology>
    


    <!-- 
    ///////////////////////////////////////////////////////////////////////////////////////
    //
    // Annotation properties
    //
    ///////////////////////////////////////////////////////////////////////////////////////
     -->

    


    <!-- http://creativecommons.org/ns#attributionName -->

    <owl:AnnotationProperty rdf:about="http://creativecommons.org/ns#attributionName"/>
    


    <!-- http://purl.org/dc/terms/date -->

    <owl:AnnotationProperty rdf:about="http://purl.org/dc/terms/date"/>
    


    <!-- http://purl.org/dc/terms/description -->

    <owl:AnnotationProperty rdf:about="http://purl.org/dc/terms/description"/>
    


    <!-- http://purl.org/dc/terms/license -->

    <owl:AnnotationProperty rdf:about="http://purl.org/dc/terms/license"/>
    


    <!-- http://purl.org/dc/terms/title -->

    <owl:AnnotationProperty rdf:about="http://purl.org/dc/terms/title"/>
    


    <!-- http://purl.org/vocab/vann/preferredNamespacePrefix -->

    <owl:AnnotationProperty rdf:about="http://purl.org/vocab/vann/preferredNamespacePrefix"/>
    


    <!-- http://purl.org/vocab/vann/preferredNamespaceUri -->

    <owl:AnnotationProperty rdf:about="http://purl.org/vocab/vann/preferredNamespaceUri"/>
    


    <!-- http://www.w3.org/2004/02/skos/core#altLabel -->

    <owl:AnnotationProperty rdf:about="http://www.w3.org/2004/02/skos/core#altLabel"/>
    


    <!-- http://www.w3.org/2004/02/skos/core#definition -->

    <owl:AnnotationProperty rdf:about="http://www.w3.org/2004/02/skos/core#definition"/>
    


    <!-- http://www.w3.org/2004/02/skos/core#note -->

    <owl:AnnotationProperty rdf:about="http://www.w3.org/2004/02/skos/core#note"/>
    


    <!-- http://www.w3.org/2004/02/skos/core#prefLabel -->

    <owl:AnnotationProperty rdf:about="http://www.w3.org/2004/02/skos/core#prefLabel"/>
    


    <!-- http://www.w3.org/2004/02/skos/core#scopeNote -->

    <owl:AnnotationProperty rdf:about="http://www.w3.org/2004/02/skos/core#scopeNote"/>
    


    <!-- 
    ///////////////////////////////////////////////////////////////////////////////////////
    //
    // Datatypes
    //
    ///////////////////////////////////////////////////////////////////////////////////////
     -->

    


    <!-- http://www.w3.org/2001/XMLSchema#date -->

    <rdfs:Datatype rdf:about="http://www.w3.org/2001/XMLSchema#date"/>
    


    <!-- http://www.w3.org/2004/02/skos/core#Concept -->

    <rdfs:Datatype rdf:about="http://www.w3.org/2004/02/skos/core#Concept"/>
    


    <!-- 
    ///////////////////////////////////////////////////////////////////////////////////////
    //
    // Object Properties
    //
    ///////////////////////////////////////////////////////////////////////////////////////
     -->

    


    <!-- http://data.europa.eu/2sa/cav#assesses -->

    <owl:ObjectProperty rdf:about="http://data.europa.eu/2sa/cav#assesses">
        <rdfs:domain rdf:resource="http://data.europa.eu/2sa/cav#Assessment"/>
        <rdfs:range rdf:resource="http://www.w3.org/ns/dcat#Resource"/>
        <rdfs:comment xml:lang="en">The reference to the asset(s) that are the object of the assessment.  (cav:Assessment -&gt; dcat:Resource (+cav:assesses)) </rdfs:comment>
        <rdfs:isDefinedBy rdf:resource="http://data.europa.eu/w21/2c930c7b-5e2f-4954-8522-bd3411339d6c"/>
        <rdfs:label xml:lang="en">Assesses</rdfs:label>
        <skos:definition xml:lang="en">The reference to the asset(s) that are the object of the assessment.  (cav:Assessment -&gt; dcat:Resource (+cav:assesses)) </skos:definition>
        <skos:prefLabel xml:lang="en">Assesses</skos:prefLabel>
    </owl:ObjectProperty>
    


    <!-- http://data.europa.eu/2sa/cav#assignedTo -->

    <owl:ObjectProperty rdf:about="http://data.europa.eu/2sa/cav#assignedTo">
        <rdfs:domain rdf:resource="http://data.europa.eu/2sa/cav#Score"/>
        <rdfs:range rdf:resource="https://data.europe.eu/semanticassets/ns/cv/cccev_v2.0.0#Criterion"/>
        <rdfs:comment xml:lang="en">The assignment of a value output to the criterion.  (cav:Score &lt;-&gt; cccev:Criterion (+cav:assignedTo +)) </rdfs:comment>
        <rdfs:isDefinedBy rdf:resource="http://data.europa.eu/w21/2c930c7b-5e2f-4954-8522-bd3411339d6c"/>
        <rdfs:label xml:lang="en">Assigned to</rdfs:label>
        <skos:definition xml:lang="en">The assignment of a value output to the criterion.  (cav:Score &lt;-&gt; cccev:Criterion (+cav:assignedTo +)) </skos:definition>
        <skos:prefLabel xml:lang="en">Assigned to</skos:prefLabel>
    </owl:ObjectProperty>
    


    <!-- http://data.europa.eu/2sa/cav#basedOn -->

    <owl:ObjectProperty rdf:about="http://data.europa.eu/2sa/cav#basedOn">
        <rdfs:domain rdf:resource="http://data.europa.eu/2sa/cav#Score"/>
        <rdfs:range rdf:resource="http://data.europa.eu/2sa/cav#EvaluationContext"/>
        <rdfs:comment xml:lang="en">The consideration of a specific evaluation context when assigning the score to a criterion. (cav:Score -&gt; cav:EvaluationContext (+cav:basedOn)) </rdfs:comment>
        <rdfs:isDefinedBy rdf:resource="http://data.europa.eu/w21/2c930c7b-5e2f-4954-8522-bd3411339d6c"/>
        <rdfs:label xml:lang="en">Based on</rdfs:label>
        <skos:definition xml:lang="en">The consideration of a specific evaluation context when assigning the score to a criterion. (cav:Score -&gt; cav:EvaluationContext (+cav:basedOn)) </skos:definition>
        <skos:prefLabel xml:lang="en">Based on</skos:prefLabel>
    </owl:ObjectProperty>
    


    <!-- http://data.europa.eu/2sa/cav#considers -->

    <owl:ObjectProperty rdf:about="http://data.europa.eu/2sa/cav#considers">
        <rdfs:domain rdf:resource="http://data.europa.eu/2sa/cav#Assessment"/>
        <rdfs:range rdf:resource="http://data.europa.eu/2sa/cav#Score"/>
        <rdfs:comment xml:lang="en">The evaluation of a criterion score in the context of the current assessment as input to issue one or more statements.</rdfs:comment>
        <rdfs:isDefinedBy rdf:resource="http://data.europa.eu/w21/2c930c7b-5e2f-4954-8522-bd3411339d6c"/>
        <rdfs:label xml:lang="en">Considers</rdfs:label>
        <skos:definition xml:lang="en">The evaluation of an assessment score as input to issue one or more statements.</skos:definition>
        <skos:prefLabel xml:lang="en">Considers</skos:prefLabel>
    </owl:ObjectProperty>
    


    <!-- http://data.europa.eu/2sa/cav#contextualisedBy -->

    <owl:ObjectProperty rdf:about="http://data.europa.eu/2sa/cav#contextualisedBy">
        <rdfs:domain rdf:resource="http://data.europa.eu/2sa/cav#Assessment"/>
        <rdfs:range rdf:resource="http://data.europa.eu/2sa/cav#Scenario"/>
        <rdfs:comment xml:lang="en">The assignment of the scenario for the current assessment providing its context, purpose and criteria.</rdfs:comment>
        <rdfs:isDefinedBy rdf:resource="http://data.europa.eu/w21/2c930c7b-5e2f-4954-8522-bd3411339d6c"/>
        <rdfs:label xml:lang="en">Contextualised by</rdfs:label>
        <skos:definition xml:lang="en">The assignment of the scenario for the current assessment providing its context, purpose and criteria.</skos:definition>
        <skos:prefLabel xml:lang="en">Contextualised by</skos:prefLabel>
    </owl:ObjectProperty>
    


    <!-- http://data.europa.eu/2sa/cav#contextualises -->

    <owl:ObjectProperty rdf:about="http://data.europa.eu/2sa/cav#contextualises">
        <rdfs:domain rdf:resource="http://data.europa.eu/2sa/cav#EvaluationContext"/>
        <rdfs:range rdf:resource="https://data.europe.eu/semanticassets/ns/cv/cccev_v2.0.0#Criterion"/>
        <rdfs:comment xml:lang="en">The provision of context for the evaluation of the criterion.</rdfs:comment>
        <rdfs:isDefinedBy rdf:resource="http://data.europa.eu/w21/2c930c7b-5e2f-4954-8522-bd3411339d6c"/>
        <rdfs:label xml:lang="en">Contextualises</rdfs:label>
        <skos:definition xml:lang="en">The provision of context for the evaluation of the criterion.</skos:definition>
        <skos:prefLabel xml:lang="en">Contextualises</skos:prefLabel>
    </owl:ObjectProperty>
    


    <!-- http://data.europa.eu/2sa/cav#definedBy -->

    <owl:ObjectProperty rdf:about="http://data.europa.eu/2sa/cav#definedBy">
        <owl:inverseOf rdf:resource="http://data.europa.eu/2sa/cav#defines"/>
        <rdfs:domain rdf:resource="http://data.europa.eu/2sa/cav#EvaluationContext"/>
        <rdfs:range rdf:resource="http://data.europa.eu/2sa/cav#Scenario"/>
        <rdfs:comment xml:lang="en">The link to the scenario that provides the evaluation context for one or more criteria</rdfs:comment>
        <rdfs:isDefinedBy rdf:resource="http://data.europa.eu/w21/2c930c7b-5e2f-4954-8522-bd3411339d6c"/>
        <rdfs:label xml:lang="en">Defined by</rdfs:label>
        <skos:definition xml:lang="en">The link to the scenario that provides the evaluation context for one or more criteria.</skos:definition>
        <skos:prefLabel xml:lang="en">Defined by</skos:prefLabel>
    </owl:ObjectProperty>
    


    <!-- http://data.europa.eu/2sa/cav#defines -->

    <owl:ObjectProperty rdf:about="http://data.europa.eu/2sa/cav#defines">
        <rdfs:domain rdf:resource="http://data.europa.eu/2sa/cav#Scenario"/>
        <rdfs:range rdf:resource="http://data.europa.eu/2sa/cav#EvaluationContext"/>
        <rdfs:comment xml:lang="en">The link to the evaluation contexts for specific criteria provided by the given scenario.</rdfs:comment>
        <rdfs:isDefinedBy rdf:resource="http://data.europa.eu/w21/2c930c7b-5e2f-4954-8522-bd3411339d6c"/>
        <rdfs:label xml:lang="en">Defines</rdfs:label>
        <skos:definition xml:lang="en">The link to the evaluation contexts for specific criteria provided by the given scenario.</skos:definition>
        <skos:prefLabel xml:lang="en">Defines</skos:prefLabel>
    </owl:ObjectProperty>
    


    <!-- http://data.europa.eu/2sa/cav#definesSub -->

    <owl:ObjectProperty rdf:about="http://data.europa.eu/2sa/cav#definesSub">
        <rdfs:domain rdf:resource="http://data.europa.eu/2sa/cav#Scenario"/>
        <rdfs:range rdf:resource="http://data.europa.eu/2sa/cav#Scenario"/>
        <rdfs:comment xml:lang="en">The definition of nested scenarios grouped based on different sub-purposes, commonalities or particularities of the sub-sets of criteria.</rdfs:comment>
        <rdfs:isDefinedBy rdf:resource="http://data.europa.eu/w21/2c930c7b-5e2f-4954-8522-bd3411339d6c"/>
        <rdfs:label xml:lang="en">Defines sub</rdfs:label>
        <skos:definition xml:lang="en">The definition of nested scenarios grouped based on different sub-purposes, commonalities or particularities of the sub-sets of criteria.</skos:definition>
        <skos:prefLabel xml:lang="en">Defines sub</skos:prefLabel>
    </owl:ObjectProperty>
    


    <!-- http://data.europa.eu/2sa/cav#documentedIn -->

    <owl:ObjectProperty rdf:about="http://data.europa.eu/2sa/cav#documentedIn">
        <rdfs:domain rdf:resource="http://data.europa.eu/2sa/cav#Asset"/>
        <rdfs:range rdf:resource="http://www.w3.org/2000/01/rdf-schema#Resource"/>
        <rdfs:comment xml:lang="en">A link to any information supporting the value of the asset and any other related relevant details.</rdfs:comment>
        <rdfs:isDefinedBy rdf:resource="http://data.europa.eu/w21/2c930c7b-5e2f-4954-8522-bd3411339d6c"/>
        <rdfs:label xml:lang="en">Documented in</rdfs:label>
        <skos:definition xml:lang="en">A link to any information supporting the value of the asset and any other related relevant details.</skos:definition>
        <skos:prefLabel xml:lang="en">Documented in</skos:prefLabel>
    </owl:ObjectProperty>
    


    <!-- http://data.europa.eu/2sa/cav#formulatedBy -->

    <owl:ObjectProperty rdf:about="http://data.europa.eu/2sa/cav#formulatedBy">
        <rdfs:domain rdf:resource="http://data.europa.eu/2sa/cav#Statement"/>
        <rdfs:range rdf:resource="http://xmlns.com/foaf/0.1/Agent"/>
        <rdfs:comment xml:lang="en">The agent(s) that issue value judgement(s) resulting from the assessment.</rdfs:comment>
        <rdfs:isDefinedBy rdf:resource="http://data.europa.eu/w21/2c930c7b-5e2f-4954-8522-bd3411339d6c"/>
        <rdfs:label xml:lang="en">Formulated by</rdfs:label>
        <skos:definition xml:lang="en">The agent(s) that issue value judgement(s) resulting from the assessment.</skos:definition>
        <skos:prefLabel xml:lang="en">Formulated by</skos:prefLabel>
    </owl:ObjectProperty>
    


    <!-- http://data.europa.eu/2sa/cav#hasInput -->

    <owl:ObjectProperty rdf:about="http://data.europa.eu/2sa/cav#hasInput">
        <rdfs:domain rdf:resource="http://data.europa.eu/2sa/cav#Score"/>
        <rdfs:range rdf:resource="http://www.w3.org/2000/01/rdf-schema#Resource"/>
        <rdfs:comment xml:lang="en">The different resources provided to feed the context for the evaluation of a criterion.</rdfs:comment>
        <rdfs:isDefinedBy rdf:resource="http://data.europa.eu/w21/2c930c7b-5e2f-4954-8522-bd3411339d6c"/>
        <rdfs:label xml:lang="en">Has input</rdfs:label>
        <skos:definition xml:lang="en">The different resources provided to feed the context for the evaluation of a criterion. </skos:definition>
        <skos:prefLabel xml:lang="en">Has input</skos:prefLabel>
    </owl:ObjectProperty>
    


    <!-- http://data.europa.eu/2sa/cav#hasReport -->

    <owl:ObjectProperty rdf:about="http://data.europa.eu/2sa/cav#hasReport">
        <rdfs:domain rdf:resource="http://data.europa.eu/2sa/cav#Assessment"/>
        <rdfs:range rdf:resource="http://www.w3.org/ns/dcat#Distribution"/>
        <rdfs:comment xml:lang="en">A manifestation of all the information related to and resulting from an assessment.</rdfs:comment>
        <rdfs:isDefinedBy rdf:resource="http://data.europa.eu/w21/2c930c7b-5e2f-4954-8522-bd3411339d6c"/>
        <rdfs:label xml:lang="en">Has report</rdfs:label>
        <skos:definition xml:lang="en">A manifestation of all the information related to and resulting from an assessment.</skos:definition>
        <skos:prefLabel xml:lang="en">Has report</skos:prefLabel>
    </owl:ObjectProperty>
    


    <!-- http://data.europa.eu/2sa/cav#hasSummary -->

    <owl:ObjectProperty rdf:about="http://data.europa.eu/2sa/cav#hasSummary">
        <rdfs:domain rdf:resource="http://data.europa.eu/2sa/cav#Assessment"/>
        <rdfs:range rdf:resource="http://www.w3.org/ns/dcat#Distribution"/>
        <rdfs:comment xml:lang="en">An abbreviated manifestation of the performed assessment.</rdfs:comment>
        <rdfs:isDefinedBy rdf:resource="http://data.europa.eu/w21/2c930c7b-5e2f-4954-8522-bd3411339d6c"/>
        <rdfs:label xml:lang="en">Has summary</rdfs:label>
        <skos:definition xml:lang="en">An abbreviated manifestation of the performed assessment.</skos:definition>
        <skos:prefLabel xml:lang="en">Has summary</skos:prefLabel>
    </owl:ObjectProperty>
    


    <!-- http://data.europa.eu/2sa/cav#includes -->

    <owl:ObjectProperty rdf:about="http://data.europa.eu/2sa/cav#includes">
        <rdfs:domain rdf:resource="http://data.europa.eu/2sa/cav#Scenario"/>
        <rdfs:range rdf:resource="https://data.europe.eu/semanticassets/ns/cv/cccev_v2.0.0#Criterion"/>
        <rdfs:comment xml:lang="en">The aggregation of criteria to one scenario or parts of it.</rdfs:comment>
        <rdfs:isDefinedBy rdf:resource="http://data.europa.eu/w21/2c930c7b-5e2f-4954-8522-bd3411339d6c"/>
        <rdfs:label xml:lang="en">Includes</rdfs:label>
        <skos:definition xml:lang="en">The aggregation of criteria to one scenario or parts of it.</skos:definition>
        <skos:prefLabel xml:lang="en">Includes</skos:prefLabel>
    </owl:ObjectProperty>
    


    <!-- http://data.europa.eu/2sa/cav#performedBy -->

    <owl:ObjectProperty rdf:about="http://data.europa.eu/2sa/cav#performedBy">
        <rdfs:domain rdf:resource="http://data.europa.eu/2sa/cav#Assessment"/>
        <rdfs:range rdf:resource="http://xmlns.com/foaf/0.1/Agent"/>
        <rdfs:comment xml:lang="en">The agent(s) that carry out the assessment.</rdfs:comment>
        <rdfs:isDefinedBy rdf:resource="http://data.europa.eu/w21/2c930c7b-5e2f-4954-8522-bd3411339d6c"/>
        <rdfs:label xml:lang="en">Performed by</rdfs:label>
        <skos:definition xml:lang="en">The agent(s) that carry out the assessment.</skos:definition>
        <skos:prefLabel xml:lang="en">Performed by</skos:prefLabel>
    </owl:ObjectProperty>
    


    <!-- http://data.europa.eu/2sa/cav#providedBy -->

    <owl:ObjectProperty rdf:about="http://data.europa.eu/2sa/cav#providedBy">
        <owl:inverseOf rdf:resource="http://data.europa.eu/2sa/cav#providesScore"/>
        <rdfs:domain rdf:resource="http://data.europa.eu/2sa/cav#Score"/>
        <rdfs:range rdf:resource="http://xmlns.com/foaf/0.1/Agent"/>
        <rdfs:comment xml:lang="en">The agent assigning the score for a given criterion as part of the assessment.</rdfs:comment>
        <rdfs:isDefinedBy rdf:resource="http://data.europa.eu/w21/2c930c7b-5e2f-4954-8522-bd3411339d6c"/>
        <rdfs:label xml:lang="en">Provided by</rdfs:label>
        <skos:definition xml:lang="en">The agent assigning the score for a given criterion as part of the assessment.</skos:definition>
        <skos:prefLabel xml:lang="en">Provided by</skos:prefLabel>
    </owl:ObjectProperty>
    


    <!-- http://data.europa.eu/2sa/cav#providesScore -->

    <owl:ObjectProperty rdf:about="http://data.europa.eu/2sa/cav#providesScore">
        <rdfs:domain rdf:resource="http://xmlns.com/foaf/0.1/Agent"/>
        <rdfs:range rdf:resource="http://data.europa.eu/2sa/cav#Score"/>
        <rdfs:comment xml:lang="en">The agent assigning the score for a given criterion as part of the assessment.</rdfs:comment>
        <rdfs:isDefinedBy rdf:resource="http://data.europa.eu/w21/2c930c7b-5e2f-4954-8522-bd3411339d6c"/>
        <rdfs:label xml:lang="en">Provides score</rdfs:label>
        <skos:definition xml:lang="en">The agent assigning the score for a given criterion as part of the assessment.</skos:definition>
        <skos:prefLabel xml:lang="en">Provides score</skos:prefLabel>
    </owl:ObjectProperty>
    


    <!-- http://data.europa.eu/2sa/cav#refersTo -->

    <owl:ObjectProperty rdf:about="http://data.europa.eu/2sa/cav#refersTo">
        <rdfs:domain rdf:resource="http://data.europa.eu/2sa/cav#Statement"/>
        <rdfs:range rdf:resource="http://data.europa.eu/2sa/cav#Scenario"/>
        <rdfs:range rdf:resource="http://data.europa.eu/2sa/cav#Score"/>
        <rdfs:range rdf:resource="https://data.europe.eu/semanticassets/ns/cv/cccev_v2.0.0#Criterion"/>
        <rdfs:comment xml:lang="en">The provision of a value judgement on one or more elements of the assessment.</rdfs:comment>
        <rdfs:isDefinedBy rdf:resource="http://data.europa.eu/w21/2c930c7b-5e2f-4954-8522-bd3411339d6c"/>
        <rdfs:label xml:lang="en">Refers to</rdfs:label>
        <skos:definition xml:lang="en">The provision of a value judgement on one or more elements of the assessment.</skos:definition>
        <skos:prefLabel xml:lang="en">Refers to</skos:prefLabel>
    </owl:ObjectProperty>
    


    <!-- http://data.europa.eu/2sa/cav#relatesTo -->

    <owl:ObjectProperty rdf:about="http://data.europa.eu/2sa/cav#relatesTo">
        <rdfs:domain rdf:resource="http://data.europa.eu/2sa/cav#EvaluationContext"/>
        <rdfs:range rdf:resource="http://www.w3.org/2000/01/rdf-schema#Resource"/>
        <rdfs:comment xml:lang="en">The resource to which a domain concept relates to.</rdfs:comment>
        <rdfs:isDefinedBy rdf:resource="http://data.europa.eu/w21/2c930c7b-5e2f-4954-8522-bd3411339d6c"/>
        <rdfs:label xml:lang="en">Relates to</rdfs:label>
        <skos:definition xml:lang="en">The resource to which a domain concept relates to.</skos:definition>
        <skos:prefLabel xml:lang="en">Relates to</skos:prefLabel>
    </owl:ObjectProperty>
    


    <!-- http://data.europa.eu/2sa/cav#requestedBy -->

    <owl:ObjectProperty rdf:about="http://data.europa.eu/2sa/cav#requestedBy">
        <rdfs:domain rdf:resource="http://data.europa.eu/2sa/cav#Assessment"/>
        <rdfs:range rdf:resource="http://xmlns.com/foaf/0.1/Agent"/>
        <rdfs:comment xml:lang="en">The agent(s) requesting the assessment of an asset.</rdfs:comment>
        <rdfs:isDefinedBy rdf:resource="http://data.europa.eu/w21/2c930c7b-5e2f-4954-8522-bd3411339d6c"/>
        <rdfs:label xml:lang="en">Requested by</rdfs:label>
        <skos:definition xml:lang="en">The agent(s) requesting the assessment of an asset.</skos:definition>
        <skos:prefLabel xml:lang="en">Requested by</skos:prefLabel>
    </owl:ObjectProperty>
    


    <!-- http://data.europa.eu/2sa/cav#resultsIn -->

    <owl:ObjectProperty rdf:about="http://data.europa.eu/2sa/cav#resultsIn">
        <rdfs:domain rdf:resource="http://data.europa.eu/2sa/cav#Assessment"/>
        <rdfs:range rdf:resource="http://data.europa.eu/2sa/cav#Statement"/>
        <rdfs:comment xml:lang="en">The creation of the statements resulting from the assessment.</rdfs:comment>
        <rdfs:isDefinedBy rdf:resource="http://data.europa.eu/w21/2c930c7b-5e2f-4954-8522-bd3411339d6c"/>
        <rdfs:label xml:lang="en">Results in</rdfs:label>
        <skos:definition xml:lang="en">The creation of the statements resulting from the assessment.</skos:definition>
        <skos:prefLabel xml:lang="en">Results in</skos:prefLabel>
    </owl:ObjectProperty>
    


    <!-- http://data.europa.eu/2sa/cav#triggeredFrom -->

    <owl:ObjectProperty rdf:about="http://data.europa.eu/2sa/cav#triggeredFrom">
        <owl:inverseOf rdf:resource="http://data.europa.eu/2sa/cav#triggers"/>
        <rdfs:domain rdf:resource="http://data.europa.eu/2sa/cav#Assessment"/>
        <rdfs:range rdf:resource="http://data.europa.eu/2sa/cav#Assessment"/>
        <rdfs:comment xml:lang="en">The event causing the current assessment as the result of another related assessment.</rdfs:comment>
        <rdfs:isDefinedBy rdf:resource="http://data.europa.eu/w21/2c930c7b-5e2f-4954-8522-bd3411339d6c"/>
        <rdfs:label xml:lang="en">Triggered from</rdfs:label>
        <skos:definition xml:lang="en">The event causing the current assessment as the result of another related assessment.</skos:definition>
        <skos:prefLabel xml:lang="en">Triggered from</skos:prefLabel>
    </owl:ObjectProperty>
    


    <!-- http://data.europa.eu/2sa/cav#triggers -->

    <owl:ObjectProperty rdf:about="http://data.europa.eu/2sa/cav#triggers">
        <rdfs:domain rdf:resource="http://data.europa.eu/2sa/cav#Assessment"/>
        <rdfs:range rdf:resource="http://data.europa.eu/2sa/cav#Assessment"/>
        <rdfs:comment xml:lang="en">The event causing further related assessment(s) due to the current one.</rdfs:comment>
        <rdfs:isDefinedBy rdf:resource="http://data.europa.eu/w21/2c930c7b-5e2f-4954-8522-bd3411339d6c"/>
        <rdfs:label xml:lang="en">Triggers</rdfs:label>
        <skos:definition xml:lang="en">The event causing further related assessment(s) due to the current one.</skos:definition>
        <skos:prefLabel xml:lang="en">Triggers</skos:prefLabel>
    </owl:ObjectProperty>
    


    <!-- http://purl.org/dc/terms/creator -->

    <owl:ObjectProperty rdf:about="http://purl.org/dc/terms/creator">
        <rdfs:domain rdf:resource="http://www.w3.org/ns/dcat#Resource"/>
        <rdfs:range rdf:resource="http://xmlns.com/foaf/0.1/Agent"/>
        <rdfs:comment xml:lang="en">The entity responsible for producing the resource.</rdfs:comment>
        <rdfs:isDefinedBy rdf:resource="https://www.dublincore.org/specifications/dublin-core/dcmi-terms/"/>
        <rdfs:label xml:lang="en">Creator</rdfs:label>
        <skos:definition xml:lang="en">The entity responsible for producing the resource.</skos:definition>
        <skos:prefLabel xml:lang="en">Creator</skos:prefLabel>
    </owl:ObjectProperty>
    


    <!-- http://purl.org/pav/previousVersion -->

    <owl:ObjectProperty rdf:about="http://purl.org/pav/previousVersion">
        <rdfs:domain rdf:resource="http://data.europa.eu/2sa/cav#Assessment"/>
        <rdfs:range rdf:resource="http://data.europa.eu/2sa/cav#Assessment"/>
        <rdfs:comment xml:lang="en">The previous version of a resource in a lineage.</rdfs:comment>
        <rdfs:isDefinedBy rdf:resource="http://purl.org/pav/"/>
        <rdfs:label xml:lang="en">Previous version</rdfs:label>
        <skos:definition xml:lang="en">The previous version of a resource in a lineage.</skos:definition>
        <skos:prefLabel xml:lang="en">Previous version</skos:prefLabel>
    </owl:ObjectProperty>
    


    <!-- http://www.w3.org/ns/dcat#distribution -->

    <owl:ObjectProperty rdf:about="http://www.w3.org/ns/dcat#distribution">
        <rdfs:domain rdf:resource="http://www.w3.org/ns/dcat#Dataset"/>
        <rdfs:range rdf:resource="http://www.w3.org/ns/dcat#Distribution"/>
        <rdfs:comment xml:lang="en">An available distribution of the dataset.</rdfs:comment>
        <rdfs:isDefinedBy rdf:resource="https://www.w3.org/ns/dcat"/>
        <rdfs:label xml:lang="en">Distribution</rdfs:label>
        <skos:definition xml:lang="en">An available distribution of the dataset.</skos:definition>
        <skos:prefLabel xml:lang="en">Distribution</skos:prefLabel>
    </owl:ObjectProperty>
    


    <!-- https://schema.org/contactPoint -->

    <owl:ObjectProperty rdf:about="https://schema.org/contactPoint">
        <rdfs:domain rdf:resource="https://schema.org/ContactPoint"/>
        <rdfs:range rdf:resource="http://www.w3.org/ns/org#Organization"/>
        <rdfs:comment xml:lang="en">A contact point for a person or organization.</rdfs:comment>
        <rdfs:isDefinedBy rdf:resource="https://schema.org/docs/schemas.html"/>
        <rdfs:label xml:lang="en">Contact Point</rdfs:label>
        <skos:definition xml:lang="en">A contact point for a person or organization.</skos:definition>
        <skos:prefLabel xml:lang="en">Contact Point</skos:prefLabel>
    </owl:ObjectProperty>
    


    <!-- 
    ///////////////////////////////////////////////////////////////////////////////////////
    //
    // Data properties
    //
    ///////////////////////////////////////////////////////////////////////////////////////
     -->

    


    <!-- http://data.europa.eu/2sa/cav#instructionDescription -->

    <owl:DatatypeProperty rdf:about="http://data.europa.eu/2sa/cav#instructionDescription">
        <rdfs:domain rdf:resource="http://data.europa.eu/2sa/cav#EvaluationContext"/>
        <rdfs:range rdf:resource="http://www.w3.org/2001/XMLSchema#string"/>
        <rdfs:comment xml:lang="en">Guideline or description that needs to followed during the evaluation of one particular criterion.</rdfs:comment>
        <rdfs:isDefinedBy rdf:resource="http://data.europa.eu/w21/2c930c7b-5e2f-4954-8522-bd3411339d6c"/>
        <rdfs:label xml:lang="en">Instruction description</rdfs:label>
        <skos:altLabel xml:lang="en">Has instruction description</skos:altLabel>
        <skos:definition xml:lang="en">Guideline or description that needs to followed during the evaluation of one particular criterion.</skos:definition>
        <skos:prefLabel xml:lang="en">Instruction description</skos:prefLabel>
    </owl:DatatypeProperty>
    


    <!-- http://data.europa.eu/2sa/cav#interpretation -->

    <owl:DatatypeProperty rdf:about="http://data.europa.eu/2sa/cav#interpretation">
        <rdfs:domain rdf:resource="http://data.europa.eu/2sa/cav#Statement"/>
        <rdfs:range rdf:resource="http://www.w3.org/2004/02/skos/core#Concept"/>
        <rdfs:comment xml:lang="en">The favourability perception of the statement (e.g. positive, negative or neutral).</rdfs:comment>
        <rdfs:isDefinedBy rdf:resource="http://data.europa.eu/w21/2c930c7b-5e2f-4954-8522-bd3411339d6c"/>
        <rdfs:label xml:lang="en">Interpretation</rdfs:label>
        <skos:altLabel xml:lang="en">Has interpretation</skos:altLabel>
        <skos:definition xml:lang="en">The favourability perception of the statement (e.g. positive, negative or neutral).</skos:definition>
        <skos:prefLabel xml:lang="en">Interpretation</skos:prefLabel>
    </owl:DatatypeProperty>
    


    <!-- http://data.europa.eu/2sa/cav#judgement -->

    <owl:DatatypeProperty rdf:about="http://data.europa.eu/2sa/cav#judgement">
        <rdfs:domain rdf:resource="http://data.europa.eu/2sa/cav#Statement"/>
        <rdfs:range rdf:resource="http://www.w3.org/2001/XMLSchema#string"/>
        <rdfs:comment xml:lang="en">The text expressing the statement’s resulting value judgement. (cav:Statement) </rdfs:comment>
        <rdfs:isDefinedBy rdf:resource="http://data.europa.eu/w21/2c930c7b-5e2f-4954-8522-bd3411339d6c"/>
        <rdfs:label xml:lang="en">Judgement</rdfs:label>
        <skos:altLabel xml:lang="en">Has judgement</skos:altLabel>
        <skos:definition xml:lang="en">The text expressing the statement’s resulting value judgement. (cav:Statement) </skos:definition>
        <skos:prefLabel xml:lang="en">Judgement</skos:prefLabel>
    </owl:DatatypeProperty>
    


    <!-- http://data.europa.eu/2sa/cav#purpose -->

    <owl:DatatypeProperty rdf:about="http://data.europa.eu/2sa/cav#purpose">
        <rdfs:domain rdf:resource="http://data.europa.eu/2sa/cav#Scenario"/>
        <rdfs:range rdf:resource="http://www.w3.org/2001/XMLSchema#string"/>
        <rdfs:comment xml:lang="en">The reason for which the assessment is done.</rdfs:comment>
        <rdfs:isDefinedBy rdf:resource="http://data.europa.eu/w21/2c930c7b-5e2f-4954-8522-bd3411339d6c"/>
        <rdfs:label xml:lang="en">Purpose</rdfs:label>
        <skos:altLabel xml:lang="en">Has purpose</skos:altLabel>
        <skos:definition xml:lang="en">The reason for which the assessment is done.</skos:definition>
        <skos:prefLabel xml:lang="en">Purpose</skos:prefLabel>
    </owl:DatatypeProperty>
    


    <!-- http://data.europa.eu/2sa/cav#status -->

    <owl:DatatypeProperty rdf:about="http://data.europa.eu/2sa/cav#status">
        <rdfs:domain rdf:resource="http://data.europa.eu/2sa/cav#Assessment"/>
        <rdfs:range rdf:resource="http://www.w3.org/2004/02/skos/core#Concept"/>
        <rdfs:comment xml:lang="en">The current situation of the assessment.</rdfs:comment>
        <rdfs:isDefinedBy rdf:resource="http://data.europa.eu/w21/2c930c7b-5e2f-4954-8522-bd3411339d6c"/>
        <rdfs:label xml:lang="en">Status</rdfs:label>
        <skos:altLabel xml:lang="en">Has label</skos:altLabel>
        <skos:definition xml:lang="en">The current situation of the assessment.</skos:definition>
        <skos:prefLabel xml:lang="en">Status</skos:prefLabel>
    </owl:DatatypeProperty>
    


    <!-- http://data.europa.eu/2sa/cav#type -->

    <owl:DatatypeProperty rdf:about="http://data.europa.eu/2sa/cav#type">
        <rdfs:comment xml:lang="en">The categorisation of the statement.</rdfs:comment>
        <rdfs:isDefinedBy rdf:resource="http://data.europa.eu/w21/2c930c7b-5e2f-4954-8522-bd3411339d6c"/>
        <rdfs:label xml:lang="en">Type</rdfs:label>
        <skos:altLabel xml:lang="en">Has type</skos:altLabel>
        <skos:definition xml:lang="en">The categorisation of the statement.</skos:definition>
        <skos:prefLabel xml:lang="en">Type</skos:prefLabel>
    </owl:DatatypeProperty>
    


    <!-- http://data.europa.eu/2sa/cav#value -->

    <owl:DatatypeProperty rdf:about="http://data.europa.eu/2sa/cav#value">
        <rdfs:domain rdf:resource="http://data.europa.eu/2sa/cav#Score"/>
        <rdfs:range rdf:resource="http://www.w3.org/2000/01/rdf-schema#Literal"/>
        <rdfs:comment xml:lang="en">The literal representing the final score assigned to one criterion.</rdfs:comment>
        <rdfs:isDefinedBy rdf:resource="http://data.europa.eu/w21/2c930c7b-5e2f-4954-8522-bd3411339d6c"/>
        <rdfs:label xml:lang="en">Value</rdfs:label>
        <skos:altLabel xml:lang="en">Has value</skos:altLabel>
        <skos:definition xml:lang="en">The literal representing the score assigned.</skos:definition>
        <skos:prefLabel xml:lang="en">Value</skos:prefLabel>
    </owl:DatatypeProperty>
    


    <!-- http://data.europa.eu/2sa/cav#valueDescription -->

    <owl:DatatypeProperty rdf:about="http://data.europa.eu/2sa/cav#valueDescription">
        <rdfs:domain rdf:resource="http://data.europa.eu/2sa/cav#Asset"/>
        <rdfs:range rdf:resource="http://www.w3.org/2001/XMLSchema#string"/>
        <rdfs:comment xml:lang="en">A text explaining the value of the resource being assessed in the context of a particular scenario.</rdfs:comment>
        <rdfs:isDefinedBy rdf:resource="http://data.europa.eu/w21/2c930c7b-5e2f-4954-8522-bd3411339d6c"/>
        <rdfs:label xml:lang="en">Value description</rdfs:label>
        <skos:altLabel xml:lang="en">Has value description</skos:altLabel>
        <skos:definition xml:lang="en">A text explaining the value of the resource being assessed in the context of a particular scenario.</skos:definition>
        <skos:prefLabel xml:lang="en">Value Description</skos:prefLabel>
    </owl:DatatypeProperty>
    


    <!-- http://purl.org/dc/terms/issued -->

    <owl:DatatypeProperty rdf:about="http://purl.org/dc/terms/issued">
        <rdfs:domain rdf:resource="http://www.w3.org/ns/dcat#Resource"/>
        <rdfs:range rdf:resource="http://www.w3.org/2001/XMLSchema#string"/>
        <rdfs:comment xml:lang="en">Recommended practice is to describe the date, date/time, or period of time as recommended for the property Date, of which this is a subproperty.</rdfs:comment>
        <rdfs:isDefinedBy rdf:resource="https://www.dublincore.org/specifications/dublin-core/dcmi-terms/"/>
        <rdfs:label xml:lang="en">Date issued</rdfs:label>
        <skos:definition xml:lang="en">Date of formal issuance of the resource.</skos:definition>
        <skos:prefLabel xml:lang="en">Date issued</skos:prefLabel>
    </owl:DatatypeProperty>
    


    <!-- http://purl.org/pav/version -->

    <owl:DatatypeProperty rdf:about="http://purl.org/pav/version">
        <rdfs:domain rdf:resource="http://data.europa.eu/2sa/cav#Assessment"/>
        <rdfs:range rdf:resource="http://www.w3.org/2001/XMLSchema#string"/>
        <rdfs:comment xml:lang="en">The version number of a resource. This is a freetext string, typical values are &quot;1.5&quot; or &quot;21&quot;. The URI identifying the previous version can be provided using prov:previousVersion.</rdfs:comment>
        <rdfs:isDefinedBy rdf:resource="http://purl.org/pav/"/>
        <rdfs:label xml:lang="en">Previous version</rdfs:label>
        <skos:definition xml:lang="en">The version number of a resource. This is a freetext string, typical values are &quot;1.5&quot; or &quot;21&quot;. The URI identifying the previous version can be provided using prov:previousVersion.</skos:definition>
        <skos:prefLabel xml:lang="en">Previous version</skos:prefLabel>
    </owl:DatatypeProperty>
    


    <!-- 
    ///////////////////////////////////////////////////////////////////////////////////////
    //
    // Classes
    //
    ///////////////////////////////////////////////////////////////////////////////////////
     -->

    


    <!-- http://data.europa.eu/2sa/cav#Assessment -->

    <owl:Class rdf:about="http://data.europa.eu/2sa/cav#Assessment">
        <rdfs:subClassOf rdf:resource="http://data.europa.eu/2sa/cav#Asset"/>
        <rdfs:comment xml:lang="en">The intellectual work to evaluate an asset against the criteria of a given scenario.</rdfs:comment>
        <rdfs:isDefinedBy rdf:resource="http://data.europa.eu/w21/2c930c7b-5e2f-4954-8522-bd3411339d6c"/>
        <rdfs:label xml:lang="en">Assessment</rdfs:label>
        <skos:definition xml:lang="en">The intellectual work to evaluate an asset against the criteria of a given scenario.</skos:definition>
        <skos:prefLabel xml:lang="en">Assessment</skos:prefLabel>
    </owl:Class>
    


    <!-- http://data.europa.eu/2sa/cav#Asset -->

    <owl:Class rdf:about="http://data.europa.eu/2sa/cav#Asset">
        <rdfs:subClassOf rdf:resource="http://www.w3.org/ns/dcat#Resource"/>
        <rdfs:comment xml:lang="en">A resource, probably resulting from a work, with purpose and value.</rdfs:comment>
        <rdfs:isDefinedBy rdf:resource="http://data.europa.eu/w21/2c930c7b-5e2f-4954-8522-bd3411339d6c"/>
        <rdfs:label xml:lang="en">Asset</rdfs:label>
        <skos:definition xml:lang="en">A resource, probably resulting from a work, with purpose and value.</skos:definition>
        <skos:prefLabel xml:lang="en">Asset</skos:prefLabel>
    </owl:Class>
    


    <!-- http://data.europa.eu/2sa/cav#EvaluationContext -->

    <owl:Class rdf:about="http://data.europa.eu/2sa/cav#EvaluationContext">
        <rdfs:comment xml:lang="en">The context for a criterion providing guidance on its evaluation considering the given scenario. This is used exceptionally to extend the context offered by the scenario when it is not sufficient for the evaluation of a given criterion. An criterion&apos;s evaluation produces an objective output that will then be considered to form value judgments expressed as the assessment&apos;s statements.</rdfs:comment>
        <rdfs:isDefinedBy rdf:resource="http://data.europa.eu/w21/2c930c7b-5e2f-4954-8522-bd3411339d6c"/>
        <rdfs:label xml:lang="en">Evaluation context</rdfs:label>
        <skos:definition xml:lang="en">The context for a criterion providing guidance on its evaluation considering the given scenario. This is used exceptionally to extend the context offered by the scenario when it is not sufficient for the evaluation of a given criterion. An criterion&apos;s evaluation produces an objective output that will then be considered to form value judgments expressed as the assessment&apos;s statements.</skos:definition>
        <skos:prefLabel xml:lang="en">Evaluation context</skos:prefLabel>
    </owl:Class>
    


    <!-- http://data.europa.eu/2sa/cav#Scenario -->

    <owl:Class rdf:about="http://data.europa.eu/2sa/cav#Scenario">
        <rdfs:subClassOf rdf:resource="http://www.w3.org/ns/dcat#Resource"/>
        <owl:disjointWith rdf:resource="http://www.w3.org/ns/dcat#Dataset"/>
        <rdfs:comment xml:lang="en">The context of the assessment establishing its purpose, the organisation of criteria being evaluated, and its reference frameworks.</rdfs:comment>
        <rdfs:isDefinedBy rdf:resource="http://data.europa.eu/w21/2c930c7b-5e2f-4954-8522-bd3411339d6c"/>
        <rdfs:label xml:lang="en">Scenario</rdfs:label>
        <skos:definition xml:lang="en">The context of the assessment establishing its purpose, the organisation of criteria being evaluated, and its reference frameworks.</skos:definition>
        <skos:prefLabel xml:lang="en">Scenario</skos:prefLabel>
    </owl:Class>
    


    <!-- http://data.europa.eu/2sa/cav#Score -->

    <owl:Class rdf:about="http://data.europa.eu/2sa/cav#Score">
        <rdfs:comment xml:lang="en">The value output assigned to the criterion as part of the assessment.</rdfs:comment>
        <rdfs:isDefinedBy rdf:resource="http://data.europa.eu/w21/2c930c7b-5e2f-4954-8522-bd3411339d6c"/>
        <rdfs:label xml:lang="en">Score</rdfs:label>
        <skos:definition xml:lang="en">The value output assigned to the criteria as part of the assessment. Additional info: This value output can be individual, and therefore per criterion or global representing the overall score of the assessment (e.g. In the case of CAMSS, assessments include two different scores).</skos:definition>
        <skos:prefLabel xml:lang="en">Score</skos:prefLabel>
    </owl:Class>
    


    <!-- http://data.europa.eu/2sa/cav#Statement -->

    <owl:Class rdf:about="http://data.europa.eu/2sa/cav#Statement">
        <rdfs:comment xml:lang="en">A value judgement, resulting from the assessment, pertinent to its entirety or to one or more of its specific parts.</rdfs:comment>
        <rdfs:isDefinedBy rdf:resource="http://data.europa.eu/w21/2c930c7b-5e2f-4954-8522-bd3411339d6c"/>
        <rdfs:label xml:lang="en">Statement</rdfs:label>
        <skos:definition xml:lang="en">A value judgement, resulting from the assessment, pertinent to its entirety or to one or more of its specific parts.</skos:definition>
        <skos:prefLabel xml:lang="en">Statement</skos:prefLabel>
    </owl:Class>
    


    <!-- http://www.w3.org/2000/01/rdf-schema#Resource -->

    <owl:Class rdf:about="http://www.w3.org/2000/01/rdf-schema#Resource"/>
    


    <!-- http://www.w3.org/ns/dcat#Dataset -->

    <owl:Class rdf:about="http://www.w3.org/ns/dcat#Dataset">
        <rdfs:subClassOf rdf:resource="http://www.w3.org/ns/dcat#Resource"/>
    </owl:Class>
    


    <!-- http://www.w3.org/ns/dcat#Distribution -->

    <owl:Class rdf:about="http://www.w3.org/ns/dcat#Distribution"/>
    


    <!-- http://www.w3.org/ns/dcat#Resource -->

    <owl:Class rdf:about="http://www.w3.org/ns/dcat#Resource"/>
    


    <!-- http://www.w3.org/ns/org#Organization -->

    <owl:Class rdf:about="http://www.w3.org/ns/org#Organization">
        <rdfs:subClassOf rdf:resource="http://xmlns.com/foaf/0.1/Agent"/>
    </owl:Class>
    


    <!-- http://xmlns.com/foaf/0.1/Agent -->

    <owl:Class rdf:about="http://xmlns.com/foaf/0.1/Agent"/>
    


    <!-- https://data.europe.eu/semanticassets/ns/cv/cccev_v2.0.0#Criterion -->

    <owl:Class rdf:about="https://data.europe.eu/semanticassets/ns/cv/cccev_v2.0.0#Criterion"/>
    


    <!-- https://schema.org/ContactPoint -->

    <owl:Class rdf:about="https://schema.org/ContactPoint"/>
</rdf:RDF>



<!-- Generated by the OWL API (version 4.5.26.2023-07-17T20:34:13Z) https://github.com/owlcs/owlapi -->

